execution/examples/EscrowSolana.v
@@ -24,11 +24,6 @@ Context {HelperTypes : ChainHelpers}.
 
 Set Nonrecursive Elimination Schemes.
 
-(* Record Setup :=
-  build_setup {
-      setup_buyer : Address;
-    }.
-
 Inductive NextStep :=
 (* Waiting for buyer to commit itemvalue * 2 *)
 | buyer_commit
@@ -37,878 +32,176 @@ Inductive NextStep :=
 (* Waiting for buyer and seller to withdraw their funds. *)
 | withdrawals
 (* No next step, sale is done. *)
-| no_next_step. *)
+| no_next_step.
 
 Record State :=
   build_state {
       last_action : nat;
-(*       next_step : NextStep; *)
-      is_initialized : bool;
+      next_step : NextStep;
+(*       is_initialized : bool; *)
       seller : Address;
-(*       buyer : Address; *)
-      seller_temp_account : Address;
-      seller_receiver : Address;
-(*       seller_withdrawable : Amount;
-      buyer_withdrawable : Amount; *)
+      buyer : Address;
+      seller_withdrawable : Amount;
+      buyer_withdrawable : Amount;
       expected_amount : Amount;
     }.
 
 MetaCoq Run (make_setters State).
 
-(* Inductive MsgType :=
-| init_escrow
+Inductive ContractInstruction :=
+| init_escrow (buyer : Address) (item_price : Amount)
 | commit_money
 | confirm_item_received
-| withdraw. *)
-
-(* Record Msg :=
-  build_message {
-    instruction : option MsgType;
-    setup : option SerializedValue;
-    amount : option SerializedValue;
-  }. *)
-
-(* Global Instance Setup_serializable : Serializable Setup :=
-  Derive Serializable Setup_rect<build_setup>.
+| withdraw.
 
 Global Instance NextStep_serializable : Serializable NextStep :=
-  Derive Serializable NextStep_rect<buyer_commit, buyer_confirm, withdrawals, no_next_step>. *)
+  Derive Serializable NextStep_rect<buyer_commit, buyer_confirm, withdrawals, no_next_step>.
 
 Global Instance State_serializable : Serializable State :=
   Derive Serializable State_rect<build_state>.
 
-(* Global Instance MsgType_serializable : Serializable MsgType :=
-  Derive Serializable MsgType_rect<init_escrow, commit_money, confirm_item_received, withdraw>.
-
-Global Instance Msg_serializable : Serializable Msg :=
-  Derive Serializable Msg_rect<build_message>. *)
+Global Instance ContractInstruction_serializable : Serializable ContractInstruction :=
+  Derive Serializable ContractInstruction_rect<init_escrow, commit_money, confirm_item_received, withdraw>.
 
 Open Scope Z.
 
-Definition escrow_init (chain : Chain) (accounts : SliceAccountInformation) (amount : Z) : result unit ProgramError :=
-  let it := new_iter accounts in
-  do seller_account <- iter_next it;
+Definition init (chain : Chain) (accounts : SliceAccountInformation) (buyer : Address) (item_price : Amount) : result unit ProgramError :=
+  let index := 0 in 
+  do seller_account <- next_account accounts index;
+  let index := 1 in
+  do escrow_account <- next_account accounts index;
   
-  do if (get_account_is_signer seller_account) then Ok tt else Err MissingRequiredSignature;
+  do if get_account_is_signer seller_account then Ok tt else Err MissingRequiredSignature;
   
-  do temp_token_account <- iter_next it;
-  do token_to_receive_account <- iter_next it;
+  (* Check rent escrow *)
+  do (exec_act (wact_special_call escrow_account (check_rent_exempt escrow_account)));
+
+  let init_state := 
+    (build_state 
+      (current_slot chain) 
+      buyer_commit 
+      (get_account_address seller_account) 
+      buyer 
+      0 0 item_price
+    ) in 
   
-  do simulate_action (wact_special_call token_to_receive_account (check_token_owner token_to_receive_account));
+  do ser_data_account init_state escrow_account;
 
-  do escrow_account <- iter_next it;
-  do simulate_action (wact_special_call escrow_account (check_rent_exempt escrow_account));
+  let expected := item_price * 2 in
+  do if (get_account_balance seller_account >? expected) then Ok tt else Err InsufficientFunds;
 
-  do escrow_info <- deser_data_account State escrow_account;
-  do if escrow_info.(is_initialized) then Err InvalidInstructionData else Ok tt;
-  
-  let new_escrow_info := escrow_info<|last_action := current_slot chain|>
-                                    <|is_initialized := true|>
-                                    <|seller := get_account_address seller_account|>
-                                    <|seller_temp_account := get_account_address temp_token_account|>
-                                    <|seller_receiver := get_account_address token_to_receive_account|>
-                                    <|expected_amount := amount|> in
-
-  do ser_data_account new_escrow_info escrow_account;
-
-  do token_program <- iter_next it;
-
-  do simulate_action (wact_special_call token_program (transfer_ownership seller_account temp_token_account seller_account));
+  (* Seller Transfer Money *)
+  do (exec_act (wact_transfer seller_account escrow_account expected));
 
   Ok tt.
 
-(* Definition escrow_init (chain : Chain) (accounts : list AccountInformation) (setup : Setup)
-  : result unit ProgramError :=
-  let buyer_address := setup_buyer setup in
+Definition buyer_commits (chain : Chain) (accounts : SliceAccountInformation) : result unit ProgramError :=
+  let index := 0 in 
+  do buyer_account <- next_account accounts index;
+  let index := 1 in
+  do escrow_account <- next_account accounts index;
 
-  let seller_account := (next_account 0 accounts NullAccount) in
-  do check_account seller_account NullAccount;
-  let temp_token_account := (next_account 1 accounts NullAccount) in
-  do check_account temp_token_account NullAccount;
-  let token_to_receive_account := (next_account 2 accounts NullAccount) in
-  do check_account token_to_receive_account NullAccount; 
-  let escrow_account := (next_account 3 accounts NullAccount) in
-  do check_account escrow_account NullAccount;
-  let rent_sysvar_account := (next_account 4 accounts NullAccount) in
-  do check_account rent_sysvar_account NullAccount;
-  let token_program_account := (next_account 5 accounts NullAccount) in
-  do check_account token_program_account NullAccount;
+  do state <- deser_data_account State escrow_account;
 
-  do if (account_is_signer seller_account) then Ok true else Err (Custom InvalidAccounts);
-  do if ((account_owner_address seller_account) =? (account_address token_program_account))%address then Ok true else Err IncorrectProgramId;
+  do if (buyer state =? get_account_address buyer_account)%address then Ok tt else Err InvalidAccountData;
 
-  let act1 := act_special_call (account_address rent_sysvar_account) (check_rent_exempt (account_address escrow_account)) in
-  do match simulate_action act1 with
-      | Ok _ => Ok true
-      | Err _ => Err (Custom InvalidInstruction)
+  do match next_step state with
+    | buyer_commit => Ok tt
+    | _ => Err InvalidInstructionData
   end;
 
-  let escrow_account_deserialize_state := ((@deserialize State _) (account_state escrow_account)) in  
-  do match escrow_account_deserialize_state with 
-      | Some st => if (is_initialized st) then Err AccountAlreadyInitialized else Ok true
-      | None => Ok true
+  let expected := (expected_amount state) * 2 in
+  do if (get_account_balance buyer_account >? expected) then Ok tt else Err InsufficientFunds;
+
+  let new_state := state<|next_step := buyer_confirm|> in
+
+  do ser_data_account new_state escrow_account;
+
+  (* Seller Transfer Money *)
+  do (exec_act (wact_transfer buyer_account escrow_account expected));
+
+  Ok tt.
+
+Definition confirm_received (chain : Chain) (accounts : SliceAccountInformation) : result unit ProgramError :=
+  let index := 0 in 
+  do buyer_account <- next_account accounts index;
+  let index := 1 in
+  do escrow_account <- next_account accounts index;
+
+  do state <- deser_data_account State escrow_account;
+
+  do if (buyer state =? get_account_address buyer_account)%address then Ok tt else Err InvalidAccountData;
+
+  do match next_step state with
+    | buyer_confirm => Ok tt
+    | _ => Err InvalidInstructionData
   end;
 
-  let act2 := act_special_call (account_address token_program_account)
-          (transfer_ownership (account_address seller_account) (account_address token_to_receive_account) (account_address token_program_account)) in
-  do match simulate_action act2 with
-      | Ok _ => Ok true
-      | Err _ => Err (Custom InvalidInstruction)
-  end;
+  let new_state := state<|next_step := withdrawals|>
+                        <|buyer_withdrawable := expected_amount state|>
+                        <|seller_withdrawable := (expected_amount state) * 3|> in
 
-  let initialized_state := (build_state
-      (current_slot chain)
-      buyer_commit
-      (account_address seller_account)
-      buyer_address
-      0 0 true)
-  in
-              
-  let escrow_account := escrow_account<|account_state := ((@serialize State _) initialized_state)|> in 
+  do ser_data_account new_state escrow_account;
 
-  let seller_account_balance := (account_balance temp_token_account) in
-  do if (buyer_address =? (account_address seller_account))%address then Err (Custom InvalidAccounts) else Ok true;
-  do if seller_account_balance =? 0 then Err (Custom InvalidAmount) else Ok true;
-  do if Z.even seller_account_balance then Ok true else Err (Custom InvalidAmount);
-
-  Ok tt. *)
+  Ok tt.
 
 
+Definition withdraw_money (chain : Chain) (accounts : SliceAccountInformation) : result unit ProgramError := 
+  let index := 0 in 
+  do withdrawer_account <- next_account accounts index;
+  let index := 1 in
+  do escrow_account <- next_account accounts index;
+  
+  do state <- deser_data_account State escrow_account;
+  let from_address := get_account_address withdrawer_account in
 
-Definition escrow_commit_money (chain : Chain) (accounts : list AccountInformation) (amount : Amount) : result (list ActionBody) EscrowError :=
-  let buyer_account_opt := (nth_error accounts 0) in
-  let temp_token_account_opt := (nth_error accounts 1) in
-  let token_to_receive_account_opt := (nth_error accounts 2) in
-  let escrow_account_opt := (nth_error accounts 3) in
-  let rent_sysvar_account_opt := (nth_error accounts 4) in
-  let token_program_account_opt := (nth_error accounts 5) in
+  match next_step state with
+    | withdrawals => 
 
-  match buyer_account_opt with
-  | Some buyer_account =>
-        match temp_token_account_opt with
-        | Some temp_token_account =>
-              match token_to_receive_account_opt with
-              | Some token_to_receive_account =>
-                  match escrow_account_opt with
-                  | Some escrow_account =>
-                      match rent_sysvar_account_opt with
-                      | Some rent_sysvar_account =>
-                          match token_program_account_opt with
-                          | Some token_program_account =>
-                              let escrow_account_deserialize_state := ((@deserialize State _) (account_state escrow_account)) in
-                              match escrow_account_deserialize_state with 
-                                | Some st => 
-                                    do if (is_initialized st) then Ok tt else Err ProgramError;
-                                    do if (buyer st =? account_address buyer_account)%address then Ok tt else Err InvalidAccounts;
+       do '(to_pay, new_state) <-
+       match from_address =? buyer state, from_address =? seller state with
+       | true, _ => Ok (buyer_withdrawable state, state<|buyer_withdrawable := 0|>)
+       | _, true => Ok (seller_withdrawable state, state<|seller_withdrawable := 0|>)
+       | _, _ => Err InvalidAccountData
+       end%address; 
 
-                                    let expected := amount * 2 in
-                                    do if (account_balance buyer_account >=? expected) then Ok tt else Err InvalidAmount;
+       do if to_pay >? 0 then Ok tt else Err InvalidInstructionData;
 
-                                    let state := st<|next_step := buyer_confirm|>
-                                                   <|last_action := current_slot chain|> in
-                                    
-                                    (* escrow_account<|account_state := (@serialize State _) initialized_state|>; *)
+       let new_state :=
+           if (buyer_withdrawable new_state =? 0) && (seller_withdrawable new_state =? 0)
+           then new_state<|next_step := no_next_step|>
+           else new_state in 
 
-                                    Ok ([])
-                                  | None => Err InvalidAccounts
-                                end
-                          | None => Err InvalidAccounts
-                          end
-                      | None => Err InvalidAccounts
-                    end
-                  | None => Err InvalidAccounts
-                  end
-              | None => Err InvalidAccounts
-              end
-        | None => Err InvalidAccounts
-        end
-  | None => Err InvalidAccounts
+       do (exec_act (wact_transfer escrow_account withdrawer_account to_pay));
+
+       do ser_data_account new_state escrow_account; 
+       Ok tt
+
+    | buyer_commit => 
+
+       do if (last_action state + 50 <? current_slot chain)%nat then Err InvalidInstructionData else Ok tt;
+       do if (from_address =? seller state)%address then Ok tt else Err InvalidAccountData;
+    
+       let new_state := state<|next_step := no_next_step|> in
+       let expected := (expected_amount state) * 2 in
+       do (exec_act (wact_transfer escrow_account withdrawer_account expected));
+       do ser_data_account new_state escrow_account;
+
+       Ok tt
+    | _ => Err InvalidInstructionData
   end.
 
-Definition escrow_confirm_item_received (chain : Chain) (accounts : list AccountInformation) (amount : Amount) : result (list ActionBody) EscrowError :=
-  let buyer_account_opt := (nth_error accounts 0) in
-  let temp_token_account_opt := (nth_error accounts 1) in
-  let token_to_receive_account_opt := (nth_error accounts 2) in
-  let escrow_account_opt := (nth_error accounts 3) in
-  let rent_sysvar_account_opt := (nth_error accounts 4) in
-  let token_program_account_opt := (nth_error accounts 5) in
 
-  match buyer_account_opt with
-  | Some buyer_account =>
-        match temp_token_account_opt with
-        | Some temp_token_account =>
-              match token_to_receive_account_opt with
-              | Some token_to_receive_account =>
-                  match escrow_account_opt with
-                  | Some escrow_account =>
-                      match rent_sysvar_account_opt with
-                      | Some rent_sysvar_account =>
-                          match token_program_account_opt with
-                          | Some token_program_account =>
-                              let escrow_account_deserialize_state := ((@deserialize State _) (account_state escrow_account)) in
-                              match escrow_account_deserialize_state with 
-                                | Some st => 
-                                    do if (is_initialized st) then Ok tt else Err ProgramError;
-                                    do if (buyer st =? account_address buyer_account)%address then Ok tt else Err InvalidAccounts;
-
-                                    let state := st<|next_step := withdrawals|>
-                                                   <|buyer_withdrawable := amount|>
-                                                   <|seller_withdrawable := amount * 3|> in
-                                    
-                                    (* escrow_account<|account_state := (@serialize State _) initialized_state|>; *)
-
-                                    Ok ([])
-                                  | None => Err InvalidAccounts
-                                end
-                          | None => Err InvalidAccounts
-                          end
-                      | None => Err InvalidAccounts
-                    end
-                  | None => Err InvalidAccounts
-                  end
-              | None => Err InvalidAccounts
-              end
-        | None => Err InvalidAccounts
-        end
-  | None => Err InvalidAccounts
+Definition escrow_process (chain : Chain) (accounts : SliceAccountInformation) (inst : option ContractInstruction) : result unit ProgramError :=
+  match inst with
+    | Some (init_escrow buyer_address item_price) => init chain accounts buyer_address item_price
+    | Some commit_money => buyer_commits chain accounts 
+    | Some confirm_item_received => confirm_received chain accounts
+    | Some withdraw => withdraw_money chain accounts
+    | _ => Err InvalidInstructionData
   end.
 
-Definition escrow_withdraw (chain : Chain) (accounts : list AccountInformation) (amount : Amount) : result (list ActionBody) EscrowError :=
-  let participant_account_opt := (nth_error accounts 0) in
-  let temp_token_account_opt := (nth_error accounts 1) in
-  let token_to_receive_account_opt := (nth_error accounts 2) in
-  let escrow_account_opt := (nth_error accounts 3) in
-  let rent_sysvar_account_opt := (nth_error accounts 4) in
-  let token_program_account_opt := (nth_error accounts 5) in
-
-  match participant_account_opt with
-  | Some participant_account =>
-        match temp_token_account_opt with
-        | Some temp_token_account =>
-              match token_to_receive_account_opt with
-              | Some token_to_receive_account =>
-                  match escrow_account_opt with
-                  | Some escrow_account =>
-                      match rent_sysvar_account_opt with
-                      | Some rent_sysvar_account =>
-                          match token_program_account_opt with
-                          | Some token_program_account =>
-                              let escrow_account_deserialize_state := ((@deserialize State _) (account_state escrow_account)) in
-                              match escrow_account_deserialize_state with 
-                                | Some st => 
-                                    do if (is_initialized st) then Ok tt else Err ProgramError;
-
-                                    match next_step st with 
-                                    | buyer_commit =>
-                                      do if (last_action st + 50 <? current_slot chain)%nat then Err ProgramError else Ok tt;
-                                      do if ((account_address participant_account) =? seller st)%address then Ok tt else Err InvalidAccounts;
-                                      let balance := account_balance escrow_account in
-                                      (* state<|next_step := no_next_step|> *)
-                                      Ok ([act_transfer (seller st) balance])
-                                    | _ =>
-
-                                      do '(to_pay, new_state) <-
-                                         match (account_address participant_account) =? (buyer st), 
-                                               (account_address participant_account) =? (seller st) with
-                                         | true, _ => Ok (buyer_withdrawable st, st<|buyer_withdrawable := 0|>)
-                                         | _, true => Ok (seller_withdrawable st, st<|seller_withdrawable := 0|>)
-                                         | _, _ => Err ProgramError
-                                         end%address;
-                                      
-                                    
-                                      do if to_pay >? 0 then Ok tt else Err ProgramError;
-                                      let new_state :=
-                                          if (buyer_withdrawable new_state =? 0) && (seller_withdrawable new_state =? 0)
-                                          then new_state<|next_step := no_next_step|>
-                                          else new_state in
-
-                                      (* escrow_account<|account_state := (@serialize State _) new_state|>; *)
-
-                                      Ok ([act_transfer (account_address participant_account) 0])
-                                    end
-                                  | None => Err InvalidAccounts
-                                end
-                          | None => Err InvalidAccounts
-                          end
-                      | None => Err InvalidAccounts
-                    end
-                  | None => Err InvalidAccounts
-                  end
-              | None => Err InvalidAccounts
-              end
-        | None => Err InvalidAccounts
-        end
-  | None => Err InvalidAccounts
-  end.
-
-Definition process (chain : Chain) (accounts : list AccountInformation) (msg : option Msg) : result (list ActionBody) EscrowError :=
-    (* TODO: Setup should come inside of the MSG *)
-    match msg with
-    | Some message =>
-        match instruction message with
-        | Some init_escrow =>
-            match setup message with
-            | Some ser_setup => 
-                match ((@deserialize Setup _) ser_setup) with 
-                | Some setup =>
-                    escrow_init chain accounts setup
-                | None => Err ProgramError
-                end
-            | None => Err ProgramError
-            end 
-        | Some commit_money => 
-            match amount message with
-            | Some ser_amount => 
-              match ((@deserialize Amount _) ser_amount) with 
-              | Some amount =>
-                  escrow_commit_money chain accounts amount
-              | None => Err ProgramError
-              end
-            | None => Err ProgramError
-            end 
-        | Some confirm_item_received =>
-            match amount message with
-            | Some ser_amount => 
-              match ((@deserialize Amount _) ser_amount) with 
-              | Some amount =>
-                escrow_confirm_item_received chain accounts amount
-              | None => Err ProgramError
-              end
-            | None => Err ProgramError
-            end 
-        | Some withdraw =>
-            match amount message with
-           | Some ser_amount => 
-             match ((@deserialize Amount _) ser_amount) with 
-              | Some amount =>
-                  escrow_withdraw chain accounts amount
-            | None => Err ProgramError
-            end
-            | None => Err ProgramError
-            end
-        | None => Err ProgramError
-        end
-    | None => Err InvalidInstruction
-    end.
-
-Definition contract : Contract Msg State :=
-  build_contract process.
-
-Section Theories.
-  Lemma no_self_calls bstate caddr :
-    reachable bstate ->
-    env_contracts bstate caddr = Some (Escrow.contract : WeakContract) ->
-    Forall (fun abody => match abody with
-                         | act_transfer to _ => (to =? caddr)%address = false
-                         | _ => False
-                         end) (outgoing_acts bstate caddr).
-  Proof.
-    contract_induction; intros; cbn in *; auto.
-    - now inversion IH.
-    - apply Forall_app; split; try tauto.
-      clear IH.
-      unfold receive in receive_some.
-      destruct_match as [[]|] in receive_some; try congruence.
-      + destruct_match in receive_some; try congruence.
-        destruct_match in receive_some; cbn in *; try congruence.
-        destruct_match in receive_some; cbn in *; try congruence.
-        inversion_clear receive_some; auto.
-      + destruct_match in receive_some; try congruence.
-        destruct_match in receive_some; cbn in *; try congruence.
-        destruct_match in receive_some; cbn in *; try congruence.
-        inversion_clear receive_some; auto.
-      + destruct_match in receive_some; try congruence.
-        * destruct_match in receive_some; cbn in *; try congruence.
-          destruct_match in receive_some; cbn in *; try congruence.
-          destruct (address_eqb_spec (ctx_from ctx) (seller prev_state)) as
-              [<-|]; cbn in *; try congruence.
-          inversion_clear receive_some.
-          constructor; try constructor.
-          apply address_eq_ne; auto.
-        * destruct_match in receive_some; cbn in *; try congruence.
-          destruct_match in receive_some; cbn in *; try congruence.
-          destruct_match in receive_some.
-          destruct_match in receive_some; cbn in *; try congruence.
-          inversion_clear receive_some.
-          constructor; try constructor.
-          apply address_eq_ne; auto.
-    - inversion_clear IH as [|? ? head_not_me tail_not_me].
-      apply Forall_app; split; auto; clear tail_not_me.
-      destruct head; try contradiction.
-      destruct action_facts as [? [? ?]].
-      destruct_address_eq; congruence.
-    - now rewrite <- perm.
-    - instantiate (DeployFacts := fun _ _ => True).
-      instantiate (CallFacts := fun _ _ _ _ => True).
-      instantiate (AddBlockFacts := fun _ _ _ _ _ _ => True).
-      unset_all; subst; cbn in *.
-      destruct_chain_step; auto.
-      destruct_action_eval; auto.
-  Qed.
-
-  Definition txs_to (to : Address) (txs : list Tx) : list Tx :=
-    filter (fun tx => (tx_to tx =? to)%address) txs.
-
-  Arguments txs_to : simpl never.
-
-  Lemma txs_to_cons addr tx txs :
-    txs_to addr (tx :: txs) =
-    if (tx_to tx =? addr)%address then
-      tx :: txs_to addr txs
-    else
-      txs_to addr txs.
-  Proof. reflexivity. Qed.
-
-  Definition txs_from (from : Address) (txs : list Tx) : list Tx :=
-    filter (fun tx => (tx_from tx =? from)%address) txs.
-
-  Arguments txs_from : simpl never.
-
-  Lemma txs_from_cons addr tx txs :
-    txs_from addr (tx :: txs) =
-    if (tx_from tx =? addr)%address then
-      tx :: txs_from addr txs
-    else
-      txs_from addr txs.
-  Proof. reflexivity. Qed.
-
-  Local Open Scope bool.
-  Definition buyer_confirmed (inc_calls : list (ContractCallInfo Msg)) buyer :=
-    existsb (fun call => (call_from call =? buyer)%address &&
-                         match call_msg call with
-                         | Some confirm_item_received => true
-                         | _ => false
-                         end) inc_calls.
-
-  Definition transfer_acts_to addr acts :=
-    filter (fun a => match a with
-                     | act_transfer to _ => (to =? addr)%address
-                     | _ => false
-                     end) acts.
-
-  Arguments transfer_acts_to : simpl never.
-
-  Lemma transfer_acts_to_cons addr act acts :
-    transfer_acts_to addr (act :: acts) =
-    if match act with
-       | act_transfer to _ => (to =? addr)%address
-       | _ => false
-       end
-    then
-      act :: transfer_acts_to addr acts
-    else
-      transfer_acts_to addr acts.
-  Proof. reflexivity. Qed.
-
-  Definition money_to
-             {bstate_from bstate_to}
-             (trace : ChainTrace bstate_from bstate_to)
-             caddr addr :=
-    sumZ tx_amount (txs_to addr (outgoing_txs trace caddr)) +
-    sumZ act_body_amount (transfer_acts_to addr (outgoing_acts bstate_to caddr)).
-
-  Lemma escrow_correct_strong bstate caddr (trace : ChainTrace empty_state bstate) :
-    env_contracts bstate caddr = Some (Escrow.contract : WeakContract) ->
-    exists (cstate : State)
-           (depinfo : DeploymentInfo Setup)
-           (inc_calls : list (ContractCallInfo Msg)),
-      deployment_info Setup trace caddr = Some depinfo /\
-      contract_state bstate caddr = Some cstate /\
-      incoming_calls Msg trace caddr = Some inc_calls /\
-      let item_worth := deployment_amount depinfo / 2 in
-      let seller_addr := deployment_from depinfo in
-      let buyer_addr := setup_buyer (deployment_setup depinfo) in
-      deployment_amount depinfo = 2 * item_worth /\
-      item_worth > 0 /\
-      seller cstate = seller_addr /\
-      buyer cstate = buyer_addr /\
-      buyer_addr <> seller_addr /\
-      forallb (fun act => match act with
-                         | act_transfer _ _ => true
-                         | _ => false
-                         end) (outgoing_acts bstate caddr) = true /\
-      match next_step cstate with
-      | buyer_commit =>
-        env_account_balances bstate caddr = 2 * item_worth /\
-        outgoing_acts bstate caddr = [] /\
-        outgoing_txs trace caddr = [] /\
-        inc_calls = []
-
-      | buyer_confirm =>
-        env_account_balances bstate caddr = 4 * item_worth /\
-        outgoing_acts bstate caddr = [] /\
-        outgoing_txs trace caddr = [] /\
-        exists origin, inc_calls = [build_call_info origin buyer_addr (2 * item_worth) (Some commit_money)]
-
-      | withdrawals =>
-        buyer_confirmed inc_calls buyer_addr = true /\
-        (exists origin, filter (fun c => negb (call_amount c =? 0)%Z ) inc_calls =
-        [build_call_info origin buyer_addr (2 * item_worth) (Some commit_money)]) /\
-        money_to trace caddr seller_addr + seller_withdrawable cstate = 3 * item_worth /\
-        money_to trace caddr buyer_addr + buyer_withdrawable cstate = 1 * item_worth
-
-      | no_next_step =>
-        buyer_confirmed inc_calls buyer_addr = true /\
-        (exists origin, filter (fun c => negb (call_amount c =? 0)%Z) inc_calls =
-        [build_call_info origin buyer_addr (2 * item_worth) (Some commit_money)]) /\
-        money_to trace caddr seller_addr = 3 * item_worth /\
-        money_to trace caddr buyer_addr = 1 * item_worth \/
-
-        (exists origin, inc_calls = [build_call_info origin seller_addr 0 (Some withdraw)]) /\
-        money_to trace caddr seller_addr = 2 * item_worth /\
-        money_to trace caddr buyer_addr = 0
-      end.
-  Proof.
-    unfold money_to.
-    contract_induction; cbn in *; intros.
-    - (* New block *)
-      auto.
-    - (* Deployment *)
-      unfold Escrow.init in *.
-      destruct (address_eqb_spec (setup_buyer setup) (ctx_from ctx));
-        cbn in *; try congruence.
-      destruct (ctx_amount ctx =? 0) eqn:amount_some; cbn in *; try congruence.
-      destruct (Z.even (ctx_amount ctx)) eqn:amount_even; cbn in *; try congruence.
-      inversion init_some; subst; clear init_some.
-      cbn.
-      assert (2 * (ctx_amount ctx / 2) > 0 -> ctx_amount ctx / 2 > 0) by lia.
-      enough (2 * (ctx_amount ctx / 2) > 0 /\
-              ctx_amount ctx = 2 * (ctx_amount ctx / 2)) by tauto.
-      assert (ctx_amount ctx mod 2 = 0).
-      {
-        rewrite Zeven_mod in amount_even.
-        unfold Zeq_bool in *.
-        destruct_match eqn:amount_mod_2 in amount_even; try congruence; auto.
-        destruct (Z.compare_spec (ctx_amount ctx mod 2) 0); auto; try congruence.
-      }
-      rewrite <- (Z_div_exact_2 (ctx_amount ctx) 2) by (auto; lia).
-      split; auto.
-      instantiate (DeployFacts := fun _ ctx => ctx_amount ctx >= 0);
-        subst DeployFacts; cbn in *.
-      apply Z.eqb_neq in amount_some.
-      lia.
-    - (* Transfer from contract to someone *)
-      repeat rewrite txs_to_cons.
-      do 5 (split; try tauto).
-      destruct IH as [_ [_ [_ [<- [_ [only_transfers IH]]]]]].
-      apply andb_prop in only_transfers.
-      split; try tauto.
-      destruct only_transfers as [is_transfer _].
-      destruct out_act; try congruence.
-      destruct tx_act_match as [<- [<- _]].
-      repeat rewrite transfer_acts_to_cons in *.
-      destruct (next_step cstate).
-      + intuition congruence.
-      + intuition congruence.
-      + (* Transfer while next_step is withdraw; so seller or buyer withdrew *)
-        do 2 (split; try tauto).
-        destruct IH as [_ [_ [? ?]]].
-        destruct_address_eq; cbn in *; lia.
-      + (* Transfer while next_step is no_next_step; action moved from queue to txs *)
-        destruct IH as [IH | IH]; [left|right].
-        * do 2 (split; try tauto).
-          destruct IH as [_ [? ?]].
-          destruct_address_eq; cbn in *; lia.
-        * split; try tauto.
-          destruct IH as [_ ?].
-          destruct_address_eq; cbn in *; lia.
-    - (* Call from someone else *)
-      do 2 (split; try tauto).
-      unfold Escrow.receive in *.
-      set (item_worth := deployment_amount dep_info / 2) in *.
-      destruct msg as [[| |]|].
-      + (* Some commit_money *)
-        destruct (next_step prev_state); try congruence.
-        destruct (address_eqb_spec (ctx_from ctx) (buyer prev_state)) as [->|];
-          cbn in *; try congruence.
-        destruct (ctx_amount ctx =? _) eqn:proper_amount in receive_some;
-          cbn in *; try congruence.
-        inversion_clear receive_some.
-        cbn.
-        do 4 (split; try tauto).
-        destruct IH as [deployed_even [_ [_ [-> [_ [_ [balance_eq [-> [-> ->]]]]]]]]].
-        apply Z.eqb_eq in proper_amount.
-        rewrite balance_eq in proper_amount.
-        rewrite proper_amount.
-        replace (ctx_contract_balance _) with (2 * item_worth + 2 * item_worth / 2 * 2) by lia.
-        rewrite <- Z.mul_comm.
-        rewrite Z.div_mul by lia.
-        repeat split;eauto.
-        lia.
-      + (* Some confirm_item_received *)
-        destruct_match in receive_some; cbn in *; try congruence.
-        destruct (address_eqb_spec (ctx_from ctx) (buyer prev_state)) as [->|];
-          cbn in *; try congruence.
-        destruct (ctx_amount ctx =? 0) eqn:zero_amount in receive_some;
-          cbn in *; try congruence.
-        inversion_clear receive_some.
-        cbn.
-        do 4 (split; try tauto).
-        destruct IH as [deployed_even [? [<- [<- [_ [_ [balance_eq [-> [-> H]]]]]]]]].
-        destruct H as [origin Hcalls].
-        rewrite Hcalls.
-        rewrite address_eq_refl.
-        cbn.
-        split; auto.
-        unfold txs_to, transfer_acts_to; cbn.
-        apply Z.eqb_eq in zero_amount.
-        rewrite zero_amount in *.
-        replace (ctx_contract_balance _) with (4 * item_worth) in * by lia.
-        rewrite (Z.mul_comm 4).
-        rewrite Z.div_mul by lia.
-        destruct (Z.eqb_spec (2 * item_worth) 0); cbn in *; try lia.
-        repeat split; eauto;lia.
-      + (* Some withdraw. Can be sent while next_step is either
-           commit_money or withdrawals. *)
-        destruct_match eqn:prev_next_step in receive_some;
-          cbn -[Nat.ltb] in *; try congruence.
-        * (* next_step was commit_money, so seller is withdrawing money
-          because buyer did not commit anything. *)
-          destruct (ctx_amount ctx =? 0) eqn:zero_amount in receive_some;
-            cbn -[Nat.ltb] in *; try congruence.
-          apply Z.eqb_eq in zero_amount.
-          rewrite zero_amount in *.
-          destruct_match in receive_some; cbn in *; try congruence.
-          destruct (address_eqb_spec (ctx_from ctx) (seller prev_state))
-            as [->|]; cbn in *; try congruence.
-          inversion_clear receive_some; cbn.
-          do 4 (split; try tauto).
-          (* In this case we go to no_next_step state without buyer having confirmed anything *)
-          right.
-          destruct IH as [_ [_ [<- [_ [? [_ [? [-> [-> ->]]]]]]]]].
-          unfold txs_to, transfer_acts_to.
-          cbn.
-          rewrite address_eq_refl, address_eq_ne by auto.
-          cbn.
-          split; eauto; lia.
-        * (* next_step was withdrawals, so either seller or buyer is withdrawing money.
-             This might put us into next_step = no_next_step. *)
-          destruct (ctx_amount ctx =? 0) eqn:zero_amount in receive_some;
-            cbn -[Nat.ltb] in *; try congruence.
-          apply Z.eqb_eq in zero_amount.
-          rewrite zero_amount in *.
-          destruct (address_eqb_spec (ctx_from ctx) (buyer prev_state))
-            as [->|]; [|destruct (address_eqb_spec (ctx_from ctx) (seller prev_state))
-                         as [->|]; cbn in *; try congruence].
-          -- (* Buyer withdrawing *)
-            cbn in *.
-            destruct_match in receive_some; cbn in *; try congruence.
-            inversion_clear receive_some; cbn.
-            apply and_assoc; split; [destruct_match; tauto|].
-            do 2 (split; try tauto).
-            destruct (Z.eqb_spec (seller_withdrawable prev_state) 0) as [seller_done|].
-            ++ (* No one has more to withdrew, next_step is no_next_step now, so establish
-                  final IH. Since we got here from withdrawal we will be in left case. *)
-              rewrite seller_done in *.
-              left.
-              repeat rewrite transfer_acts_to_cons.
-              fold (buyer_confirmed prev_inc_calls
-                                    (setup_buyer (deployment_setup dep_info))).
-              destruct IH as [_ [_ [<- [-> [? [_ [-> [[? ->] [? ?]]]]]]]]].
-              rewrite address_eq_refl.
-              rewrite address_eq_ne by assumption.
-              cbn.
-              do 2 (split; [eauto|]).
-              lia.
-            ++ (* Seller still has more to withdraw, next_step is still withdrawals *)
-              cbn.
-              rewrite prev_next_step.
-              repeat rewrite transfer_acts_to_cons.
-              fold (buyer_confirmed prev_inc_calls
-                                    (setup_buyer (deployment_setup dep_info))).
-              destruct IH as [_ [_ [<- [-> [? [_ [-> [[? ->] [? ?]]]]]]]]].
-              rewrite address_eq_refl.
-              rewrite address_eq_ne by assumption.
-              cbn.
-              do 2 (split; eauto).
-              lia.
-          -- (* Seller withdrawing. Todo: generalize and clean up. *)
-            cbn in *.
-            destruct_match in receive_some; cbn in *; try congruence.
-            inversion_clear receive_some; cbn.
-            apply and_assoc; split; [destruct_match; tauto|].
-            do 2 (split; try tauto).
-            destruct (Z.eqb_spec (buyer_withdrawable prev_state) 0) as [buyer_done|].
-            ++ (* No one has more to withdrew, next_step is no_next_step now, so establish
-                  final IH. Since we got here from withdrawal we will be in left case. *)
-              rewrite buyer_done in *.
-              left.
-              repeat rewrite transfer_acts_to_cons.
-              fold (buyer_confirmed prev_inc_calls
-                                    (setup_buyer (deployment_setup dep_info))).
-              destruct IH as [_ [_ [<- [<- [? [_ [-> [[? ->] [? ?]]]]]]]]].
-              rewrite address_eq_refl.
-              rewrite address_eq_ne by auto.
-              cbn.
-              do 2 (split; eauto).
-              lia.
-            ++ (* Buyer still has more to withdraw, next_step is still withdrawals *)
-              cbn.
-              rewrite prev_next_step.
-              repeat rewrite transfer_acts_to_cons.
-              fold (buyer_confirmed prev_inc_calls
-                                    (setup_buyer (deployment_setup dep_info))).
-              destruct IH as [_ [_ [<- [<- [? [_ [-> [[? ->] [? ?]]]]]]]]].
-              rewrite address_eq_refl.
-              rewrite address_eq_ne by auto.
-              cbn.
-              do 2 (split; eauto).
-              lia.
-      + (* None *)
-        congruence.
-    - (* Self call *)
-      instantiate (CallFacts := fun _ ctx _ _ => ctx_from ctx <> ctx_contract_address ctx);
-        subst CallFacts; cbn in *; congruence.
-    - (* Permuting queue *)
-      do 5 (split; try tauto).
-      split.
-      + now rewrite <- perm.
-      + assert (out_queue = [] -> out_queue' = [])
-          by (intros ->; now apply Permutation_nil).
-        unfold transfer_acts_to in *.
-        repeat rewrite sumZ_filter in *.
-        destruct (next_step cstate); try tauto.
-        * now rewrite <- perm.
-        * destruct IH as [_ [_ [_ [_ [_ [_ [IH | IH]]]]]]];
-            [left|right]; rewrite <- perm; auto.
-    - instantiate (AddBlockFacts := fun _ _ _ _ _ _ => True).
-      unset_all; subst; cbn in *.
-      destruct_chain_step; auto.
-      destruct_action_eval; auto.
-      intros.
-      pose proof (no_self_calls bstate_from to_addr ltac:(assumption) ltac:(assumption))
-           as all.
-      unfold outgoing_acts in *.
-      rewrite queue_prev in *.
-      subst act; cbn in all.
-      destruct_address_eq; cbn in *; auto.
-      inversion_clear all as [|? ? hd _].
-      destruct msg.
-      + contradiction.
-      + rewrite address_eq_refl in hd.
-        congruence.
-  Qed.
-
-  Definition net_balance_effect
-             {bstate_from bstate_to : ChainState}
-             (trace : ChainTrace bstate_from bstate_to)
-             (caddr addr : Address) : Amount :=
-    sumZ tx_amount (txs_to addr (outgoing_txs trace caddr))
-    - sumZ tx_amount (txs_from addr (incoming_txs trace caddr)).
-
-  (* Our main assumption is that the escrow will always finish due to
-  economically rational actors. We do not formalize this. *)
-  Definition is_escrow_finished cstate :=
-    match next_step cstate with
-    | no_next_step => true
-    | _ => false
-    end.
-
-  (* The functional correctness of the Escrow, under the assumption that the
-  escrow finishes due to rational actors. *)
-  Corollary escrow_correct
-            {ChainBuilder : ChainBuilderType}
-            prev new header acts :
-    builder_add_block prev header acts = Ok new ->
-    let trace := builder_trace new in
-    forall caddr,
-      env_contracts new caddr = Some (Escrow.contract : WeakContract) ->
-      exists (depinfo : DeploymentInfo Setup)
-             (cstate : State)
-             (inc_calls : list (ContractCallInfo Msg)),
-        deployment_info Setup trace caddr = Some depinfo /\
-        contract_state new caddr = Some cstate /\
-        incoming_calls Msg trace caddr = Some inc_calls /\
-        let item_worth := deployment_amount depinfo / 2 in
-        let seller := deployment_from depinfo in
-        let buyer := setup_buyer (deployment_setup depinfo) in
-        is_escrow_finished cstate = true ->
-        (buyer_confirmed inc_calls buyer = true /\
-         net_balance_effect trace caddr seller = item_worth /\
-         net_balance_effect trace caddr buyer = -item_worth \/
-
-         buyer_confirmed inc_calls buyer = false /\
-         net_balance_effect trace caddr seller = 0 /\
-         net_balance_effect trace caddr buyer = 0).
-  Proof.
-    intros after_add trace caddr escrow_at_caddr.
-    cbn in *.
-    pose proof (escrow_correct_strong _ caddr trace escrow_at_caddr) as general.
-    cbn in general.
-    destruct general as
-        [cstate [depinfo [inc_calls [? [? [? [? [? [? [? [? [_ IH]]]]]]]]]]]].
-    exists depinfo, cstate, inc_calls.
-    do 3 (split; [tauto|]).
-    intros is_finished.
-    unfold is_escrow_finished in *.
-    destruct (next_step cstate); try congruence; clear is_finished.
-    unfold net_balance_effect, money_to.
-    assert (inc_txs:
-              forall addr,
-                sumZ tx_amount (txs_from addr (incoming_txs trace caddr)) =
-                sumZ (fun '(a, b, c) => c)
-                     (filter (fun '(from, _, _) => (from =? addr)%address)
-                             (map (fun tx => (tx_from tx, tx_to tx, tx_amount tx))
-                                  (incoming_txs trace caddr)))).
-    {
-      intros addr.
-      induction (incoming_txs trace caddr) as [|hd tl IH'].
-      - reflexivity.
-      - rewrite txs_from_cons.
-        cbn.
-        destruct_address_eq; cbn in *; rewrite IH'; reflexivity.
-    }
-
-    repeat rewrite inc_txs; clear inc_txs.
-    rewrite (incoming_txs_contract caddr _ trace _ depinfo _ inc_calls) by assumption.
-    repeat rewrite filter_app, sumZ_app.
-    cbn.
-    rewrite address_eq_refl.
-    rewrite address_eq_ne by auto.
-    cbn.
-    rewrite 2!filter_map, 2!sumZ_map.
-
-    set (buyer_addr := setup_buyer (deployment_setup depinfo)) in *.
-    set (seller_addr := deployment_from depinfo) in *.
-
-    unfold money_to, transfer_acts_to in IH.
-    cbn in IH.
-
-    change (fun a => call_amount a) with (@call_amount _ Msg).
-
-    destruct IH as [IH | IH]; [left|right].
-    - split; [tauto|].
-      destruct IH as [_ [[origin HH] ?]].
-      remember (build_call_info _ _ _ (Some commit_money)) as commitment.
-      assert (Hsum :
-                forall f,
-                  sumZ call_amount (filter f inc_calls) =
-                  sumZ call_amount (filter f [commitment])).
-      {
-        intros f.
-        rewrite <- HH.
-        clear -inc_calls.
-        induction inc_calls as [|hd tl IH']; auto.
-        cbn.
-        destruct (Z.eqb_spec (call_amount hd) 0) as [zero_amount|].
-        - cbn.
-          destruct (f hd); cbn; try rewrite zero_amount; rewrite IH'; auto.
-        - cbn.
-          destruct (f hd); cbn; rewrite IH'; auto.
-      }
-
-      rewrite 2!Hsum; clear Hsum; subst commitment; cbn in *.
-      rewrite address_eq_refl, address_eq_ne by auto.
-      cbn.
-      split; lia.
-    - destruct IH as [[? ->] IH].
-      cbn.
-      rewrite address_eq_refl, address_eq_ne by auto.
-      cbn.
-      split; [auto|].
-      split; lia.
-  Qed.
-
-End Theories.
+Definition contract : Contract ContractInstruction State :=
+  build_contract escrow_process.
 
 End EscrowSolana.
